qa/lean/Ragu.lean
@@ -11,7 +11,8 @@ import Ragu.Instances.Element.Alloc
 import Ragu.Instances.Element.AllocSquare
 import Ragu.Instances.Element.DivNonzero
 import Ragu.Instances.Element.Fold
-import Ragu.Instances.Element.EnforceRootOfUnity
+import Ragu.Instances.Element.EnforceRootOfUnityK2
+import Ragu.Instances.Element.EnforceRootOfUnityK5
 import Ragu.Instances.Element.EnforceZero
 import Ragu.Instances.Element.Invert
 import Ragu.Instances.Element.InvertWith
