qa/lean/Ragu/Instances/Element/EnforceRootOfUnityK2.lean
@@ -1,0 +1,42 @@
+import Ragu.Circuits.Element.EnforceRootOfUnity
+import Ragu.Instances.Autogen.Element.EnforceRootOfUnityK2
+import Ragu.Core
+
+namespace Ragu.Instances.Element.EnforceRootOfUnityK2
+open Ragu.Instances.Autogen.Element.EnforceRootOfUnityK2
+
+def deserializeInput (input : Vector (Expression (F p)) inputLen) : Var field (F p) :=
+  input[0]
+
+def serializeOutput (_output : Var unit (F p)) : Vector (Expression (F p)) 0 :=
+  #v[]
+
+def formal_instance : Core.Statements.FormalInstance where
+  p
+  exportedOperations
+  exportedOutput
+
+  deserializeInput
+  serializeOutput
+
+  reimplementation := (Circuits.Element.EnforceRootOfUnity.circuit 2).isGeneralFormalCircuit.toWithHint
+
+  same_constraints := by
+    intro input
+    simp [Core.Statements.FlatOperation.eraseCompute, List.map,
+      Operations.toFlat, circuit_norm,
+      FormalAssertion.isGeneralFormalCircuit,
+      GeneralFormalCircuit.toWithHint,
+      GeneralFormalCircuit.WithHint.toSubcircuit, FormalCircuit.toSubcircuit,
+      deserializeInput, exportedOperations,
+      Circuits.Element.EnforceRootOfUnity.circuit,
+      Circuits.Element.EnforceRootOfUnity.elaborated,
+      Circuits.Element.EnforceRootOfUnity.main,
+      Circuits.Element.EnforceRootOfUnity.squareIter,
+      Circuits.Element.Mul.circuit, Circuits.Element.Mul.elaborated, Circuits.Element.Mul.main]
+    constructor
+  same_output := by
+    intro input
+    rfl
+
+end Ragu.Instances.Element.EnforceRootOfUnityK2
